% coding:utf-8
\section{Vektoren}
\subsection{Aufgabe 1}
\[  \]
\[  \]
\[  \]

\subsection{Aufgabe 2}
\[  \]
\[  \]
\[  \]

\subsection{Aufgabe 3}
\[  \]
\[  \]
\[  \]

\section{Folgen}
\subsection{Aufgabe 1}
\[ a_n = a_1 + (n - 1)d \]
\[ d = a_{n+1} - a_n \]
\[ \frac{a_{n_2} - a_{n_1}}{n_2 - n_1} = d  \]
\[ \underline{\underline{a_{n_3} = a_{n_2} + d \cdot (n_3 - n_2) = a_{n_1} + d \cdot (n_3 - n_1)}} \]

\subsection{Aufgabe 2}
a)
\[ \underline{\underline{a_n = a_1 \cdot q^{n-1}}} \]
b)
\[ \underline{\underline{b_n = b_0 \cdot q^{n}}} \]
c)
\[ q = \left(\frac{c_{n_2}}{c_{n_1}}\right)^{\frac{1}{n_2 - n_1}} \quad\left( = \sqrt[(n_2 - n_1)]{\frac{c_{n_2}}{c_{n_1}}}\right) \]
\[ \underline{\underline{c_{n_3} = c_{n_2} \cdot q^{n_3 - n_2} = c_{n_1} \cdot q^{n_3 - n_1}}} \]
Achtung: Wenn $n_2 - n_1$ gerade ist, dann ist das Vorzeichen des Ergebnisses evtl. nicht definiert. 

\subsection{Aufgabe 3}
\[ q = \frac{a_{n+1}}{a_n} = \frac{a_2}{a_1} \]
\[ a_n = a_1 \cdot q^{n - 1} \]
\[ \frac{a_n}{a_1} = q^{n - 1} \]
\[ n - 1 = \log_q \left(\frac{a_n}{a_1}\right) \]
\[ \underline{\underline{n = \log_q \left(\frac{a_n}{a_1}\right) + 1}}\]

\subsection{Aufgabe 4}
\[  \]
\[  \]
\[  \]

\section{Reihen}
\subsection{Aufgabe 1}
\[  \]
\[  \]
\[  \]

\subsection{Aufgabe 2}
\[  \]
\[  \]
\[  \]

\subsection{Aufgabe 3}
\[  \]
\[  \]
\[  \]

\subsection{Aufgabe 4}
\[  \]
\[  \]
\[  \]
